CollapsingTowers/Stlc/Basic.lean
@@ -7,10 +7,6 @@ inductive Expr : Type where
   | app (f : Expr) (arg : Expr)
   | unit
 
-inductive value : Expr -> Prop where
-  | value_lam : value (.lam e)
-  | value_unit : value .unit
-
 @[simp]
 def fv : Expr → Finset ℕ
   | .bvar _ => ∅
